new/sequence.v
@@ -1,0 +1,82 @@
+Require Import braun log insert util index list.
+Require Import Arith Arith.Even Arith.Div2 List.
+Require Import Program.
+Require Import Omega.
+
+Section sequence.
+  Variable A : Set.
+
+  Inductive SequenceR : bin_tree A -> list A -> Prop :=
+    | SR_mt :
+        SequenceR (bt_mt A) nil
+    | SR_node :
+        forall x s t ss ts,
+          SequenceR s ss ->
+          SequenceR t ts ->
+          SequenceR (bt_node x s t) (x::interleave A ss ts).
+  Hint Constructors SequenceR.
+
+  Lemma BraunR_SequenceR :
+    forall b n,
+      Braun b n ->
+      forall l,
+        SequenceR b l ->
+        n = (length l).
+  Proof.
+    intros b n B.
+    induction B; intros l SR; invclr SR.
+    auto.
+
+    rename H into BP.
+    rename H4 into SRs.
+    rename H5 into SRt.
+    apply IHB1 in SRs.
+    apply IHB2 in SRt.
+    subst.
+    rewrite interleave_length_split.
+    simpl.
+    omega.
+  Qed.
+
+  Theorem SequenceR_IndexR :
+    forall b i x,
+      IndexR A b i x ->
+      forall xs,
+        Braun b (length xs) ->
+        SequenceR b xs ->
+        ListIndexR A xs i x.
+  Proof.
+    intros b i x IR.
+    induction IR; intros xs BP SR; invclr SR; eauto;
+    rename H3 into SRs; rename H4 into SRt.
+
+    eapply LIR_zero.
+
+    invclr BP.
+    rename H3 into BP.
+    rename H4 into Bs.
+    rename H5 into Bt.
+    rename H2 into EQ.
+    rewrite <- interleave_length_split in EQ.
+    replace s_size with (length ss) in *; try omega.
+    replace t_size with (length ts) in *; try omega.
+    apply IHIR in SRs; eauto.
+    apply ListIndexR_interleave_evens; eauto.
+    symmetry. eapply BraunR_SequenceR. apply Bs.
+    apply SRs.
+
+    invclr BP.
+    rename H3 into BP.
+    rename H4 into Bs.
+    rename H5 into Bt.
+    rename H2 into EQ.
+    rewrite <- interleave_length_split in EQ.
+    replace s_size with (length ss) in *; try omega.
+    replace t_size with (length ts) in *; try omega.
+    apply IHIR in SRt; eauto.
+    apply ListIndexR_interleave_odds; eauto.
+    symmetry. eapply BraunR_SequenceR. apply Bs.
+    apply SRs.
+  Qed.
+
+End sequence.
